First (uncomplete) version of lucas with tree-number

num/Lucas.v
@@ -1,12 +1,150 @@
 Set Implicit Arguments.
 
+Require Import PZAux.
 Require Import ZArith.
+Require Import ZDivModAux.
 Require Import Basic_type.
 Require Import ZnZ.
 Require Import Zn2Z.
 Require Import Mod_op.
-Require Import W8_op.
+Require Import W2_op.
 Require Import W.
+Require Import LucasLehmer.
+
+Open Scope Z_scope. 
+
+Section test.
+
+Variable w: Set.
+Variable w_op: znz_op w.
+Variable op_spec: znz_spec w_op.
+Variable p: positive.
+Variable b: w.
+
+Notation "[| x |]" :=
+   (znz_to_Z w_op x)  (at level 0, x at level 99).
+
+Hypothesis p_more_1: 2 < Zpos p.
+Hypothesis b_p: [|b|] = 2 ^ Zpos p - 1.
+
+Lemma b_pos: 0 < [|b|].
+rewrite b_p; auto with zarith.
+assert (2 ^ 0 < 2 ^ Zpos p); auto with zarith.
+apply PZAux.Zpower_lt_monotone; auto with zarith.
+rewrite PZAux.Zpower_exp_0 in H; auto with zarith.
+Qed.
+
+Hint Resolve b_pos.
+
+Variable m_op: mod_op w.
+Variable m_op_spec: mod_spec w_op b m_op.
+
+Let w2 := m_op.(add_mod) w_op.(znz_1) w_op.(znz_1).
+
+Lemma w1_b: [|w_op.(znz_1)|] = 1 mod [|b|].
+rewrite (spec_1 op_spec); simpl; auto.
+rewrite Zmod_def_small; auto with zarith.
+split; auto with zarith.
+rewrite b_p.
+assert (2 ^ 1 < 2 ^ Zpos p); auto with zarith.
+apply PZAux.Zpower_lt_monotone; auto with zarith.
+rewrite PZAux.Zpower_exp_1 in H; auto with zarith.
+Qed.
+
+Lemma w2_b: [|w2|] = 2 mod [|b|].
+unfold w2; rewrite (add_mod_spec m_op_spec _ _ _ _ w1_b w1_b).
+rewrite w1_b; rewrite <- Zmod_plus; auto with zarith.
+Qed.
+
+Let w4 := m_op.(add_mod) w2 w2.
+
+Lemma w4_b: [|w4|] = 4 mod [|b|].
+unfold w4; rewrite (add_mod_spec m_op_spec _ _ _ _ w2_b w2_b).
+rewrite w2_b; rewrite <- Zmod_plus; auto with zarith.
+Qed.
+
+Let square_m2 :=
+   let square := m_op.(square_mod) in
+   let sub := m_op.(sub_mod) in
+   fun x => sub (square x) w2.
+
+Definition lucastest :=
+ w_op.(znz_to_Z) (iter_pos (Pminus p 2) _ square_m2 w4).
+
+Theorem lucastest_aux_correct:
+ forall p1 z n, 0 <= n -> [|z|] = fst (s n) mod (2 ^ Zpos p - 1) ->
+       [|iter_pos p1 _ square_m2 z|] = fst (s (n + Zpos p1)) mod (2 ^ Zpos p - 1).
+intros p1; pattern p1; apply Pind; simpl iter_pos; simpl s; clear p1.
+intros z p1 Hp1 H.
+unfold square_m2.
+rewrite <- b_p in H.
+generalize (square_mod_spec m_op_spec _ _ H); intros H1.
+rewrite (sub_mod_spec m_op_spec _ _ _ _ H1 w2_b).
+rewrite H1; rewrite w2_b; auto with zarith.
+rewrite H; rewrite <- Zmod_mult; auto with zarith.
+rewrite <- Zmod_minus; auto with zarith.
+rewrite sn; simpl; auto with zarith.
+rewrite b_p; auto.
+intros p1 Rec w1 z Hz Hw1.
+rewrite Pplus_one_succ_l; rewrite iter_pos_plus;
+ simpl iter_pos.
+match goal with |- context[square_m2 ?X] =>
+  set (tmp := X); unfold square_m2; unfold tmp; clear tmp
+end.
+generalize (Rec _ _ Hz Hw1); intros H1.
+rewrite <- b_p in H1.
+generalize (square_mod_spec m_op_spec _ _ H1); intros H2.
+rewrite (sub_mod_spec m_op_spec _ _ _ _ H2 w2_b).
+rewrite H2; rewrite w2_b; auto with zarith.
+rewrite H1; rewrite <- Zmod_mult; auto with zarith.
+rewrite <- Zmod_minus; auto with zarith.
+replace (z + Zpos (1 + p1)) with ((z + Zpos p1) + 1); auto with zarith.
+rewrite sn; simpl fst; try rewrite b_p; auto with zarith.
+rewrite Zpos_plus_distr; auto with zarith.
+Qed.
+
+Theorem lucastest_prop: lucastest = fst(s (Zpos p -2)) mod (2 ^ Zpos p - 1).
+unfold lucastest.
+assert (F: 0 <= 0); auto with zarith.
+generalize (lucastest_aux_correct (p -2) w4 F); simpl Zplus;
+   rewrite Zpos_minus; auto with zarith.
+intros tmp; apply tmp; clear tmp.
+rewrite <- b_p; simpl; exact w4_b.
+Qed.
+
+Theorem lucastest_prop_cor: lucastest = 0 -> (2 ^ Zpos p - 1 | fst(s (Zpos p - 2))).
+intros H.
+apply Zmod_divide.
+assert (H1: 2 ^ 1 < 2 ^ Zpos p); auto with zarith.
+apply PZAux.Zpower_lt_monotone; auto with zarith.
+rewrite PZAux.Zpower_exp_1 in H1; auto with zarith.
+apply trans_equal with (2:= H); apply sym_equal; apply lucastest_prop; auto.
+Qed.
+
+Theorem lucastest_prime:  lucastest = 0 -> prime (2 ^ Zpos p - 1).
+intros H1; case (prime_dec (2 ^ Zpos p - 1)); auto; intros H2.
+case Zdivide_div_prime_le_square with (2 := H2).
+assert (H3: 2 ^ 1 < 2 ^ Zpos p); auto with zarith.
+apply PZAux.Zpower_lt_monotone; auto with zarith.
+rewrite PZAux.Zpower_exp_1 in H3; auto with zarith.
+intros q (H3, (H4, H5)).
+contradict H5; apply Zlt_not_le.
+generalize q_more_than_square; unfold Mp; intros tmp; apply tmp;
+  auto; clear tmp.
+apply lucastest_prop_cor; auto.
+case (Zle_lt_or_eq 2 q); auto.
+apply prime_le_2; auto.
+intros H5; subst.
+absurd (2 <= 1); auto with arith.
+apply Zdivide_le; auto with zarith.
+case H4; intros x Hx.
+exists (2 ^ (Zpos p -1) - x).
+rewrite Zmult_minus_distr_r; rewrite <- Hx; unfold Mp.
+pattern 2 at 2; rewrite <- Zpower_exp_1; rewrite <- Zpower_exp; auto with zarith.
+replace (Zpos p - 1 + 1) with (Zpos p); auto with zarith.
+Qed.
+
+End test.
 
 Definition znz_of_Z (w:Set) (op:znz_op w) z :=
  match z with
@@ -14,20 +152,149 @@ Definition znz_of_Z (w:Set) (op:znz_op w) z :=
  | _ => op.(znz_0)
  end.
 
-Definition lucastest (w:Set) (op:znz_op w) p :=
+Fixpoint plength (p: positive) : positive :=
+  match p with 
+    xH => xH
+  | xO p1 => Psucc (plength p1)
+  | xI p1 => Psucc (plength p1)
+  end.
+
+Definition lucas p :=
+ let op := cmk_op (nat_of_P (plength p) - 1) in
  let b := znz_of_Z op (Zpower 2 (Zpos p) - 1) in
+ let mod_op := mmake_mod_op op b p (2 * op.(znz_digits) - p) in
+  lucastest op p mod_op.
+
+Time Eval compute in lucas 127.
+
+Theorem plength_correct: forall p, (Zpos p < 2 ^ Zpos (plength p))%Z.
+assert (F: (forall p, 2 ^ (Zpos (Psucc p)) = 2 * 2 ^ Zpos p)%Z).
+intros p; replace (Zpos (Psucc p)) with (1 + Zpos p)%Z.
+rewrite Zpower_exp; auto with zarith.
+rewrite Zpos_succ_morphism; unfold Zsucc; auto with zarith.
+intros p; elim p; simpl plength; auto.
+intros p1 Hp1; rewrite F; repeat rewrite Zpos_xI.
+assert (tmp: (forall p, 2 * p = p + p)%Z); 
+  try repeat rewrite tmp; auto with zarith.
+intros p1 Hp1; rewrite F; rewrite (Zpos_xO p1).
+assert (tmp: (forall p, 2 * p = p + p)%Z); 
+  try repeat rewrite tmp; auto with zarith.
+rewrite ZPowerAux.Zpower_exp_1; auto with zarith.
+Qed.
+
+Theorem plength_pred_correct: forall p, (Zpos p <= 2 ^ Zpos (plength (Ppred p)))%Z.
+intros p; case (Psucc_pred p); intros H1.
+subst; simpl plength.
+rewrite ZPowerAux.Zpower_exp_1; auto with zarith.
+pattern p at 1; rewrite <- H1.
+rewrite Zpos_succ_morphism; unfold Zsucc; auto with zarith.
+generalize (plength_correct (Ppred p)); auto with zarith.
+Qed.
+
+Definition pheight p := plength (Ppred (plength (Ppred p))).
+
+Theorem pheight_correct: forall p, (Zpos p <= 2 ^ (2 ^ (Zpos (pheight p))))%Z.
+intros p; apply Zle_trans with (1 := (plength_pred_correct p)).
+apply ZPowerAux.Zpower_le_monotone; auto with zarith.
+split; auto with zarith.
+unfold pheight; apply plength_pred_correct.
+Qed.
+
+Axiom ok: forall P, P.
+
+Theorem lucas_prime:
+ forall p, 2 < Zpos p -> lucas p = 0 -> prime (2 ^ Zpos p - 1).
+unfold lucas; intros p Hp H.
+ match type of H with lucastest ?x ?y ?z = _ =>
+   generalize (lucastest_prime x)
+ end.
+generalize lucastest_prime.
+intros H1; case (prime_de
+ forall m, (1 < Zpos m) ->
+ let op := cmk_op (nat_of_P (plength m)) in
+ let b := znz_of_Z op (Zpower 2 (Zpos m) - 1) in
  let mod_op := make_mod_op op b in
  let w2 := op.(znz_add) op.(znz_1) op.(znz_1) in
  let w4 := op.(znz_add) w2 w2 in
  let square_m2 :=
    let square := mod_op.(square_mod) in
    let sub := mod_op.(sub_mod) in
-   fun x => sub (square x) w2   
- in
- op.(znz_to_Z) (iter_pos (Pminus p 2) _ square_m2 w4).
+   fun x => sub (square x) w2   in
+ let z1 := op.(znz_to_Z) b
+ in forall p z2 n, 0 <= n -> op.(znz_to_Z) z2 = fst (s n) mod z1 ->
+       op.(znz_to_Z) (iter_pos p _ square_m2 z2) = fst (s (n + Zpos p)) mod z1.
+intros m Hm op b mod_op w2 w4 square_m2 z1 p.
+assert (F: 1 < znz_to_Z op b).
+unfold b.
+apply ok.
+pattern p; apply Pind; simpl.
+intros z2 n Hn H; rewrite sn; simpl.
+unfold square_m2.
+generalize (@make_mod_spec _ op b F).
+new_mod_spec
+assert (F: znz_to_Z op (square_mod mod_op z2) = fst (s n) mod z1).
+intros z1 z2 n Hn H H1; rewrite sn; auto; rewrite H1;  rewrite Zmodd_correct; rewrite
+ Zsquare_correct; simpl.
+unfold Zminus; rewrite Zmod_plus; auto.
+rewrite (Zmod_plus (fst (s n) * fst (s n))); auto with zarith.
+eq_tac; auto.
+eq_tac; auto.
+apply sym_equal; apply Zmod_mult; auto.
+intros n Rec z1 z2 n1 Hn1 H1 H2.
+rewrite Pplus_one_succ_l; rewrite iter_pos_plus.
+rewrite Rec with (n0 := n1); auto.
+replace (n1 + Zpos (1 + n)) with ((n1 + Zpos n) + 1); auto with zarith.
+rewrite sn; simpl; try rewrite Zmodd_correct; try rewrite Zsquare_correct; simpl; aut
+o with zarith.
+unfold Zminus; rewrite Zmod_plus; auto.
+unfold Zmodd.
+rewrite (Zmod_plus (fst (s (n1 + Zpos n)) * fst (s (n1 + Zpos n)))); auto with zarith
+.
+eq_tac; auto.
+eq_tac; auto.
+apply sym_equal; apply Zmod_mult; auto.
+rewrite Zpos_plus_distr; auto with zarith.
+Qed.
 
+Theorem SS_prop: forall n, 1 < n -> SS n = fst(s (n -2)) mod (Mp n).
+intros n Hn; unfold SS.
+cut (0 <= n - 2); auto with zarith.
+case (n - 2).
+intros _; rewrite Zmodd_correct; rewrite s0; auto.
+intros p1 H2; rewrite SS_aux_correct with (n := 0); auto with zarith.
+apply Zle_lt_trans with 1; try apply mersenne_pos; auto with zarith.
+rewrite Zmodd_correct; rewrite s0; auto.
+intros p1 H2; case H2; auto.
+Qed.
 
-  
+Theorem SS_prop_cor: forall p, 1 < p -> SS p = 0 -> (Mp p | fst(s (p -2))).
+intros p H H1.
+apply Zmod_divide.
+apply Zlt_gt; apply Zlt_trans with 1; try apply mersenne_pos; auto with zarith.
+apply trans_equal with (2:= H1); apply sym_equal; apply SS_prop; auto.
+Qed.
+
+Theorem LucasLehmer:  forall p, 2 < p -> SS p = 0 -> prime (Mp p).
+intros p H H1; case (prime_dec (Mp p)); auto; intros H2.
+case Zdivide_div_prime_le_square with (2 := H2).
+apply mersenne_pos; apply Zlt_trans with 2; auto with zarith.
+intros q (H3, (H4, H5)).
+contradict H5; apply Zlt_not_le.
+apply q_more_than_square; auto.
+apply SS_prop_cor; auto.
+apply Zlt_trans with 2; auto with zarith.
+case (Zle_lt_or_eq 2 q); auto.
+apply prime_le_2; auto.
+intros H5; subst.
+absurd (2 <= 1); auto with arith.
+apply Zdivide_le; auto with zarith.
+case H4; intros x Hx.
+exists (2 ^ (p -1) - x).
+rewrite Zmult_minus_distr_r; rewrite <- Hx; unfold Mp.
+pattern 2 at 2; rewrite <- Zpower_exp_1; rewrite <- Zpower_exp; auto with zarith.
+replace (p - 1 + 1) with p; auto with zarith.
+Qed.
+*)
 Time Eval vm_compute in lucastest w1024_op 521.
 (* sans square : Finished transaction in 8. secs (7.66u,0.01s) *)
 (* Finished transaction in 6. secs (5.74u,0.01s) *)
